src/program_proof/wal/circ_proof.v
@@ -1244,19 +1244,6 @@ Proof.
   iApply ("HΦ" with "[$]").
 Qed.
 
-Definition block0: Block :=
-  list_to_vec (replicate (Z.to_nat 4096) (U8 0)).
-
-Lemma replicate_zero_to_block0 :
-  replicate (int.nat 4096) (zero_val byteT) =
-  Block_to_vals block0.
-Proof.
-  change (zero_val byteT) with #(U8 0).
-  change (int.nat 4096) with (Z.to_nat 4096).
-  rewrite /Block_to_vals /block0.
-  reflexivity.
-Qed.
-
 Theorem circ_low_wf_empty logblocks :
   length logblocks = Z.to_nat LogSz ->
   circ_low_wf (replicate (Z.to_nat LogSz) (U64 0)) logblocks.
