src/program_proof/buftxn/sep_buftxn_recovery_proof.v
@@ -38,7 +38,7 @@ Section goose_lang.
     dom (gset _) dinit = list_to_set (seqZ 513 sz) →
     dom (gset _) kinds = list_to_set (U64 <$> (seqZ 513 sz)) →
     (513 + Z.of_nat sz) * block_bytes * 8 < 2^64 →
-    0 d↦∗ repeat circ_proof.block0 513 ∗ 513 d↦∗ repeat circ_proof.block0 sz -∗
+    0 d↦∗ repeat block0 513 ∗ 513 d↦∗ repeat block0 sz -∗
   |={⊤}=> ∃ γ, let logm0 := Build_async (kind_heap0 kinds) [] in
                is_txn_durable γ dinit logm0 ∗
                txn_durable γ 0 ∗
